\documentclass{article}
\usepackage[utf8]{inputenc}
\usepackage[a4paper, total={6in, 8in}]{geometry}
\usepackage{amsmath, amssymb, amsthm}

\newtheorem{theorem}{Theorem}

\newtheorem*{lemma}{Lemma}
\newtheorem*{definition}{Definition}
\newtheorem*{corollary}{Corollary}
\newtheorem*{axiom}{Axiom}

\newcommand{\N}{\mathbb{N}}
\newcommand{\Z}{\mathbb{Z}}
\newcommand{\Q}{\mathbb{Q}}
\newcommand{\R}{\mathbb{R}}
\newcommand{\C}{\mathbb{C}}

\begin{document}

\section{Axioms for the natural numbers}

\begin{axiom}
	\textbf{(Peano Postulates).} There exists a set $\N$ with an element $1 \in \N$ and a function $s: \N \rightarrow \N$ that satisfy the following three properties.
	\begin{enumerate}
		\item[a.] There is no $n \in \N$ such that $s(n) = 1$.
		\item[b.] The function is injective.
		\item[c.] Let $G \subseteq \N$ be a set. Suppose that $1 \in G$ and that if $g \in G$ then $s(g) \in G$. Then $G = \N$.
	\end{enumerate}
\end{axiom}

\begin{definition}
	The set of \textbf{natural numbers}, denoted $\N$, is the set the existence of which is given in the Peano Postulates.
\end{definition}

\begin{theorem}
	\textbf{(Definition by Recursion).} Let $H$ be a set, and let $e \in H$ and let $k: H \rightarrow H$ be a function. Then there is a unique function $f: \N \rightarrow H$ such that $f(1) = e$ and that $f \circ s = k \circ f$.
\end{theorem}

\begin{theorem}
	There is a unique binary operation $+: \N \times \N \rightarrow \N$ that satisfies the following two properties for all $n,m \in \N$.
	\begin{enumerate}
		\item[a.] $n + 1 = s(n)$
		\item[b.] $n + s(m) = s(n + m)$
	\end{enumerate}
\end{theorem}

\begin{theorem}
	There is a unique binary operation $\cdot : \N \times \N \rightarrow \N$ that satisfies the following two properties for all $n,m \in \N$.
	\begin{enumerate}
		\item[a.] $n \cdot 1 = n$
		\item[b.] $n \cdot s(m) = (n \cdot m) + n$
	\end{enumerate}
\end{theorem}

\begin{theorem}
	Let $a, b, c \in \N$.
	\begin{enumerate}
		\item If $a + c = b + c$ then $a = b$ (Cancellation Law for Addition).
		\item $(a + b) + c = a + (b + c)$ (Associative Law for Addition).
		\item $1 + a = s(a) = a + 1$.
		\item $a + b = b + a$ (Commutative Law for Addition).
		\item $a + b \ne 1$.
		\item $a + b \ne a$.
		\item $a \cdot 1 = a = 1\cdot a$ (Identity Law for Multiplication).
		\item $(a + b)c = ac + bc$ (Distributive Law).
		\item $ab = ba$ (Commutative Law for Multiplication).
		\item $c(a + b) = ca + cb$ (Distributive Law)
		\item $(ab)c = a(bc)$ (Associative Law for Multiplication).
		\item If $ac = bc$ then $a = b$ (Cancellation Law for Multiplication).
		\item $ab = 1$ if and only if $a = 1 = b$.
	\end{enumerate}
\end{theorem}

\begin{definition}
	The relation $<$ on $\N$ is defined by $a < b$ if and only if there is some $p \in \N$ such that $a + p = b$ for all $a,b \in \N$. The relation $\le$ on $\N$ is defined by $a \le b$ if and only if $a < b$ or $a = b$, for all $a, b \in \N$.
\end{definition}

\begin{theorem}
	Let $a,b,c,d \in \N$.
	\begin{enumerate}
		\item $a \le a$ and $a \nless a$, and $a < a + 1$.
		\item $1 \le a$.
		\item If $a < b$ and $b < c$, then $a < c$; if $a \le b$ and $b < c$ then $a < c$; if $a < b$ and $b \le c$ then $a < c$; if $a \le b$ and $b \le c$ then $a \le c$.
		\item $a < b$ if and only if $a + c < b + c$.
		\item $a < b$ if and only if $ac < bc$.
		\item Precisely one of $a < b$ or $a = b$ or $a > b$ holds (Trichotomy Law).
		\item $a \le b$ or $b \le a$
		\item If $a \le b$ and $b \le a$ then $a = b$.
		\item It cannot be that $b < a < b + 1$.
		\item $a \le b$ if and only if $a < b + 1$.
		\item $a < b$ if and only if $a + 1 \le b$.
	\end{enumerate}
\end{theorem}

\begin{theorem}
	\textbf{(Well-Ordering Principle).} Let $G \subseteq \N$ be a non-empty set. Then there is some $m \in G$ such that $m \le g$ for all $g \in G$.
\end{theorem}

\subsection*{Exercises}

\subsubsection*{1. Fill in the missing details in the proof of Theorem 1.2.6.}

\begin{proof}
	To prove uniqueness, suppose that there are two binary operations $\cdot$ and $\times$ on $\N$ that satisfy the two properties of the theorem. Let \[G = \left\{x \in \N | n \cdot x = n \times x \text{ for all } n \in N\right\}.\]
	Then $G \subseteq N$. By part (a) applied to both $\cdot$ and $\times$ we see that $n \cdot 1 = 1 = n \times 1$ for all $n \in \N$, so $1 \in G$. Now let $q \in G$ and $n \in N$. Then $n \cdot q = n \times q$. Then it follows from part (b) that \[n \cdot s(q) = (n \cdot q) + n = (n \times q) + n = n \times s(q).\] Then $s(q) \in G$, and therefore we can conclude using part (c) of the Peano Postulates that $G = \N$.

	Let $q \in \N$. Let $h_q: \N \mapsto \N$ be defined by $h_q(m) = m + q$ for all $m \in \N$. Applying theorem 1.2.4 to the set $\N$, the element $q \in \N$ and the function $h_q: \N \mapsto \N$ implies that there is a unique function $g_q: \N \mapsto \N$ such that $g_q(1) = q$ and $g_q \circ s = h_q \circ g_q$. Let $\cdot: \N \times \N \mapsto \N$ be defined by $c \cdot d = g_c(d)$ for all $(c,d)\in \N \times \N$. Let $n,m \in \N$. Then $n \cdot 1 = g_n(1) = n$ which is part (a), and $n \cdot s(m) = g_n(s(m)) = (g_n \circ s)(m) = (h_n \circ g_n)(m) = h_n(g_n(m)) = (n \cdot m) + n$ which is part (b).
\end{proof}

\subsubsection*{2. Prove Theorem 1.2.7 (2, 3, 4, 7, 8, 9, 10, 11, 13)}

\begin{enumerate}
	\item[2.] $(a + b) + c = a + (b + c)$
	\begin{proof}
		Let \[G = \left\{z\in \N: \text{ if } x,y \in \N \text, (x + y) + z = x + (y + z)\right\}.\]
		Then $(x + y) + 1 = s(x + y) = x + s(y) = x + (y + 1)$, so $1 \in G$.
		Now, let $z \in G$. Then 
		\begin{align*}
			(x + y) + s(z) &= (x + y) + (z + 1) \\&= ((x + y) + z) + 1 \\&= (x + (y + z)) + 1 \\&= x + ((y + z) + 1) \\&= x + (y + (z + 1)) \\&= x + (y + s(z))
		\end{align*}
		So if $z \in G$ then $s(z) \in G$, and therefore $G = \N$.
	\end{proof}
	\item[3.] $1 + a = s(a) = a + 1$.
	\begin{proof}
		It follows from the definition of +, that $a + 1 = s(a)$. Let $G = \left\{a \in N: 1 + a = s(a)\right\}$. $1 + 1 = s(1)$, so $1 \in G$. Now, let $a \in G$. Then $(1 + a) + 1 = s(1 + a) = 1 + s(a) = 1 + (1 + a)$. So $s(a) \in G$, and therefore $G = \N$.
	\end{proof}
	\item[4.] $a + b = b + a$
	\begin{proof}
		Let \[G = \left\{a \in \N: \text{ if } b \in \N, a + b = b + a \right\}.\]
		Let $b \in N$. It follows that $1 + b = b + 1$, so $1 \in G$. Now, let $a \in G$. Then \[(a + 1) + b = (1 + a) + b = 1 + (a + b) = 1 + (b + a) = (b + a) + 1 = b + (a + 1).\] So $s(a) \in G$, and therefore $G = \N$.
	\end{proof}
	\item[7.] $a \cdot 1 = a = 1 \cdot a$
	\begin{proof}
		It follows from the definition of $\cdot$ that $a \cdot 1 = a$. Let $G = \left\{a \in \N: 1 \cdot a = a\right\}$. Since $1 \cdot 1 = 1$, we know that $1 \in G$. Let $a \in G$. Then \[1 \cdot s(a) = (1 \cdot a) + 1 = a + 1 = s(a).\] So $s(a) \in \N$, and therefore $G = \N$.
	\end{proof}
	\item[8.] $(a + b)c = ac + bc$
	\begin{proof}
		Let $G \left\{c \in \N: \text{ if } a,b \in \N, \text{ then }(a + b)c = ac + bc\right\}$.
		We know that $(a + b) \cdot 1 = a + b = a \cdot 1 + b \cdot 1$, so $1 \in G$.
		Let $c \in \N$. Then \[(a + b) \cdot s(c) = (a + b) \cdot c + (a + b) = ac + bc + a + b = (ac + a) + (bc + b) = a \cdot s(c) + b \cdot s(c).\] So $s(c) \in G$, and therefore $G = \N$.
	\end{proof}
	\item[9. ] $ab = ba$
	\begin{proof}
		Let $G = \left\{a \in \N: \text{ if } b \in \N, \text{ then }ab = ba\right\}$. We've shown in (7) that $1 \cdot b = b \cdot 1$, so $1 \in G$. Let $a \in G$. Then \[ b \cdot s(a) = b \cdot (a + 1) = ba + b = ab + 1 \cdot b = (a + 1) \cdot b = s(a) \cdot b. \] So $s(a) \in G$, and therefore $G = \N$.
	\end{proof}
	\item[10. ] $c(a + b) = ca + cb$
	\begin{proof}
		Based on (9) and (8), we know that $(a + b) = ac + bc = ca + cb$ and $(a + b)c = c(a + b)$, so $c(a + b) = ca + cb$.
	\end{proof}
	\item[11. ] $(ab)c = a(bc)$
	\begin{proof}
		Let $G = \left\{c \in \N: \text{ if } a,b \in \N, \text{ then } (ab)c = a(bc)\right\}$. Since $(ab)\cdot 1 = ab = a(b \cdot 1)$, $1 \in G$. Now let $c \in G$. Then \[ (ab)\cdot s(c) = (ab)(c + 1) = (ab)c + ab = a(bc) + ab = a(bc + b) = a(b(c + 1)) = a(b \cdot s(c)). \] Then $s(c) \in G$, so $G = \N$.
	\end{proof}
	\item[13. ] $ab = 1 \text{ if and only if } a = 1 = b$.
	\begin{proof}
		If $a = 1 = b$, it is obvious that $ab = 1$. Suppose that $ab = 1$, and let $b \ne 1$. Then there exists such $c \in \N$ that $c + 1 = b$. Then \[ab = a \cdot (c + 1) = ac + a = 1. \] This contradicts point (5) of the theorem ($a + b \ne 1$). Then $b = 1$, and $1 = ab = a \cdot 1 = a$, so $a = 1 = b$.
	\end{proof}
\end{enumerate}

\subsubsection*{3. Let $a, b \in \N$. Suppose that $a < b$. Prove that there is a unique $p \in \N$ such that $a + p = b$.}

\begin{proof}
	From the definition of $<$, we know that $a < b$ if and only if there is some $p \in N$ such that $a + p = b$ for all $a,b \in \N$.
	Let $q,p \in \N$, such that $a + p = b$ and $a + q = b$. Then $a + p = a + q$, so $p = q$, so $p$ is unique.
\end{proof}


\end{document}